Commit for now

Lambda.thy
@@ -2,6 +2,13 @@ theory Lambda
   imports Main
 begin
 
+smt_status help
+
+datatype lam
+  = LVar string
+  | LApp lam lam (infix "°⇩λ" 200)
+  | LAbs string lam ("λ⇩λ_. _" 300)
+
 datatype db
   = Var nat
   | App db db (infix "°" 200)
@@ -12,17 +19,46 @@ primrec lift :: "db ⇒ nat ⇒ db" where
 | lift_App: "lift (m ° n) k = lift m k ° lift n k"
 | lift_Abs: "lift (λm) k = λlift m (k+1)"
 
+primrec lam_to_db' :: "lam ⇒ (string ⇒ nat) ⇒ db" where
+  "lam_to_db' (LVar x) σ = Var (σ x)"
+| "lam_to_db' (m °⇩λ n) σ = (lam_to_db' m σ) ° (lam_to_db' n σ)"
+| "lam_to_db' (λ⇩λx. m) σ = λlift (lam_to_db' m (σ(x:=0))) 0"
+
+definition lam_to_db :: "lam ⇒ db" where
+  "lam_to_db x = lam_to_db' x (λ_. 0)"
+
+value "lam_to_db ((λ⇩λ''y''. (λ⇩λ''x''. (LVar ''y''))) °⇩λ (λ⇩λ''x''. LVar ''x''))"
+
 primrec subst :: "db ⇒ nat ⇒ db ⇒ db" ("_[_::=_]" [300, 0, 0] 300) where
-  lift_Var: "(Var i)[k::=e] = (if k < i then Var (i-1) else
+  subst_Var: "(Var i)[k::=e] = (if k < i then Var (i-1) else
                                if k = i then e else Var i)"
-| lift_App: "(m ° n)[k::=e] = m[k::=e] ° n[k::=e]"
-| lift_Abs: "(λ m)[k::=e] = λ(m[k+1::=lift e 0])"
+| subst_App: "(m ° n)[k::=e] = m[k::=e] ° n[k::=e]"
+| subst_Abs: "(λ m)[k::=e] = λ(m[k+1::=lift e 1])"
 
 inductive beta :: "db ⇒ db ⇒ bool" (infix "→⇩β" 50) where
-  appL: "m →⇩β m' ⟹ m ° n →⇩β m' ° n"
-| appR: "n →⇩β n' ⟹ m ° n →⇩β m ° n'"
-| abs: "m →⇩β m' ⟹ (λm) →⇩β λm'"
-| beta: "(λm) ° n →⇩β m[0::=n]"
+  beta_appL: "m →⇩β m' ⟹ m ° n →⇩β m' ° n"
+| beta_appR: "n →⇩β n' ⟹ m ° n →⇩β m ° n'"
+| beta_abs: "m →⇩β m' ⟹ (λm) →⇩β λm'"
+| beta_beta: "(λm) ° n →⇩β m[1::=n]"
+
+abbreviation beta_reds :: "db ⇒ db ⇒ bool" (infix "→⇩β⇧*" 50) where
+  "m →⇩β⇧* m' == beta⇧*⇧* m m'"
+
+theorem
+  shows "∃m'. lam_to_db m →⇩β⇧* m' ∧ lam_to_db ((λ⇩λx. LVar x) °⇩λ m) →⇩β⇧* m'"
+proof (induct m)
+  case (LVar x)
+  have "lam_to_db (LVar y) = Var 0" by (simp add: lam_to_db_def)
+  have "lam_to_db ((λ⇩λx. LVar x) °⇩λ LVar y) = (λVar 1) ° Var 0" by (simp add: lam_to_db_def)
+  then show ?case
+    apply (auto simp add: lam_to_db_def beta_beta)
+next
+  case (LApp m1 m2)
+  then show ?case sorry
+next
+  case (LAbs x1a m)
+  then show ?case sorry
+qed
 
 code_pred (modes: i ⇒ o ⇒ bool as reduce') beta .
 
